cava/Cava/Extraction.v
@@ -34,8 +34,11 @@ Require Import Cava.Monad.CombinationalMonad.
 Require Import Cava.Monad.CavaClass.
 Require Import Cava.Monad.Combinators.
 Require Import Cava.Monad.NetlistGeneration.
-Require Import Cava.Monad.UnsignedAdders.
 Require Import Cava.Monad.XilinxAdder.
+
+Require Import Cava.Lib.BitVectorOps.
+Require Import Cava.Lib.FullAdder.
+Require Import Cava.Lib.UnsignedAdders.
 
 Recursive Extraction Library BitArithmetic.
 Recursive Extraction Library Cava.
@@ -74,4 +77,6 @@ Recursive Extraction Library VectorUtils.
 Recursive Extraction Library UnsignedAdders.
 Recursive Extraction Library XilinxAdder.
 
-
+Recursive Extraction Library BitVectorOps.
+Recursive Extraction Library FullAdder.
+Recursive Extraction Library UnsignedAdders.
